common/theories/Universes.v
@@ -1,7 +1,7 @@
 From Stdlib Require Import OrdersAlt Structures.OrdersEx MSetList MSetAVL MSetFacts MSetProperties MSetDecide FMapAVL.
 From Equations Require Import Equations.
 From MetaRocq.Utils Require Import utils MRMSets MRFSets NonEmptyLevelExprSet.
-From MetaRocq.Common Require Import BasicAst config.
+From MetaRocq.Common Require Import BasicAst config UnivConstraintType.
 From Stdlib Require Import ssreflect.
 
 Local Open Scope nat_scope.
@@ -628,50 +628,6 @@ Proof.
   - intros le. rewrite val_singleton. lia.
   - intros le x. rewrite val_add. lia.
 Qed.
-
-Module ConstraintType.
-  Inductive t_ : Set := Le | Eq.
-  Derive NoConfusion EqDec for t_.
-
-  Definition t := t_.
-  Definition eq : t -> t -> Prop := eq.
-  Definition eq_equiv : Equivalence eq := _.
-
-  Inductive lt_ : t -> t -> Prop :=
-  | LeEq : lt_ Le Eq.
-  Derive Signature for lt_.
-  Definition lt := lt_.
-
-  Global Instance lt_strorder : StrictOrder lt.
-  Proof.
-    constructor.
-    - intros []; intro X; inversion X.
-    - intros ? ? ? X Y; invs X; invs Y; constructor.
-  Qed.
-
-  Global Instance lt_compat : Proper (eq ==> eq ==> iff) lt.
-  Proof.
-    intros ? ? X ? ? Y; invs X; invs Y. reflexivity.
-  Qed.
-
-  Definition compare (x y : t) : comparison :=
-    match x, y with
-    | Le, Le => Datatypes.Eq
-    | Le, Eq => Datatypes.Lt
-    | Eq, Eq => Datatypes.Eq
-    | Eq, _  => Datatypes.Gt
-    end.
-
-  Lemma compare_spec x y : CompareSpec (eq x y) (lt x y) (lt y x) (compare x y).
-  Proof.
-    destruct x, y; repeat constructor.
-  Qed.
-
-  Lemma eq_dec x y : {eq x y} + {~ eq x y}.
-  Proof.
-    unfold eq. decide equality.
-  Qed.
-End ConstraintType.
 
 Module UnivConstraint.
   Definition t : Type := Universe.t * ConstraintType.t * Universe.t.
